Translation/Conversion.v
@@ -318,6 +318,48 @@ Inductive red1 (Σ : sglobal_context) : sterm -> sterm -> Prop :=
     red1 Σ pB pB' ->
     red1 Σ (sCongSum B1 B2 pA pB) (sCongSum B1 B2 pA pB')
 
+(** CongPi1 *)
+| congpi1_red_ty_l B1 B1' B2 pA pB pp :
+    red1 Σ B1 B1' ->
+    red1 Σ (sCongPi1 B1 B2 pA pB pp) (sCongPi1 B1' B2 pA pB pp)
+
+| congpi1_red_ty_r B1 B2 B2' pA pB pp :
+    red1 Σ B2 B2' ->
+    red1 Σ (sCongPi1 B1 B2 pA pB pp) (sCongPi1 B1 B2' pA pB pp)
+
+| congpi1_red_tm_dom B1 B2 pA pA' pB pp :
+    red1 Σ pA pA' ->
+    red1 Σ (sCongPi1 B1 B2 pA pB pp) (sCongPi1 B1 B2 pA' pB pp)
+
+| congpi1_red_tm_cod B1 B2 pA pB pB' pp :
+    red1 Σ pB pB' ->
+    red1 Σ (sCongPi1 B1 B2 pA pB pp) (sCongPi1 B1 B2 pA pB' pp)
+
+| congpi1_red_tm_tm B1 B2 pA pB pp pp' :
+    red1 Σ pp pp' ->
+    red1 Σ (sCongPi1 B1 B2 pA pB pp) (sCongPi1 B1 B2 pA pB pp')
+
+(** CongPi2 *)
+| congpi2_red_ty_l B1 B1' B2 pA pB pp :
+    red1 Σ B1 B1' ->
+    red1 Σ (sCongPi2 B1 B2 pA pB pp) (sCongPi2 B1' B2 pA pB pp)
+
+| congpi2_red_ty_r B1 B2 B2' pA pB pp :
+    red1 Σ B2 B2' ->
+    red1 Σ (sCongPi2 B1 B2 pA pB pp) (sCongPi2 B1 B2' pA pB pp)
+
+| congpi2_red_tm_dom B1 B2 pA pA' pB pp :
+    red1 Σ pA pA' ->
+    red1 Σ (sCongPi2 B1 B2 pA pB pp) (sCongPi2 B1 B2 pA' pB pp)
+
+| congpi2_red_tm_cod B1 B2 pA pB pB' pp :
+    red1 Σ pB pB' ->
+    red1 Σ (sCongPi2 B1 B2 pA pB pp) (sCongPi2 B1 B2 pA pB' pp)
+
+| congpi2_red_tm_tm B1 B2 pA pB pp pp' :
+    red1 Σ pp pp' ->
+    red1 Σ (sCongPi2 B1 B2 pA pB pp) (sCongPi2 B1 B2 pA pB pp')
+
 (** CongEq *)
 | congeq_red_eq_ty pA pu pv pA' :
     red1 Σ pA pA' ->
