Translation/ITyping.v
@@ -192,6 +192,37 @@ Inductive typing (Σ : sglobal_context) : scontext -> sterm -> sterm -> Prop :=
     sHeq (sSort (max_sort s z)) (sSum nx A1 B1)
          (sSort (max_sort s z)) (sSum ny A2 B2)
 
+| type_CongPi1 Γ s z nx ny A1 A2 B1 B2 p1 p2 pA pB pp :
+    Σ ;;; Γ |-i pA : sHeq (sSort s) A1 (sSort s) A2 ->
+    Σ ;;; Γ ,, (sPack A1 A2)
+    |-i pB : sHeq (sSort z) ((lift 1 1 B1){ 0 := sProjT1 (sRel 0) })
+                 (sSort z) ((lift 1 1 B2){ 0 := sProjT2 (sRel 0) }) ->
+    Σ ;;; Γ |-i pp : sHeq (sSum nx A1 B1) p1 (sSum ny A2 B2) p2 ->
+    Σ ;;; Γ |-i A1 : sSort s ->
+    Σ ;;; Γ |-i A2 : sSort s ->
+    Σ ;;; Γ ,, A1 |-i B1 : sSort z ->
+    Σ ;;; Γ ,, A2 |-i B2 : sSort z ->
+    Σ ;;; Γ |-i p1 : sSum nx A1 B1 ->
+    Σ ;;; Γ |-i p2 : sSum ny A2 B2 ->
+    Σ ;;; Γ |-i sCongPi1 B1 B2 pA pB pp : sHeq A1 (sPi1 A1 B1 p1)
+                                              A2 (sPi1 A2 B2 p2)
+
+| type_CongPi2 Γ s z nx ny A1 A2 B1 B2 p1 p2 pA pB pp :
+    Σ ;;; Γ |-i pA : sHeq (sSort s) A1 (sSort s) A2 ->
+    Σ ;;; Γ ,, (sPack A1 A2)
+    |-i pB : sHeq (sSort z) ((lift 1 1 B1){ 0 := sProjT1 (sRel 0) })
+                 (sSort z) ((lift 1 1 B2){ 0 := sProjT2 (sRel 0) }) ->
+    Σ ;;; Γ |-i pp : sHeq (sSum nx A1 B1) p1 (sSum ny A2 B2) p2 ->
+    Σ ;;; Γ |-i A1 : sSort s ->
+    Σ ;;; Γ |-i A2 : sSort s ->
+    Σ ;;; Γ ,, A1 |-i B1 : sSort z ->
+    Σ ;;; Γ ,, A2 |-i B2 : sSort z ->
+    Σ ;;; Γ |-i p1 : sSum nx A1 B1 ->
+    Σ ;;; Γ |-i p2 : sSum ny A2 B2 ->
+    Σ ;;; Γ |-i sCongPi2 B1 B2 pA pB pp :
+               sHeq (B1{ 0 := sPi1 A1 B1 p1}) (sPi2 A1 B1 p1)
+                    (B2{ 0 := sPi1 A2 B2 p2}) (sPi2 A2 B2 p2)
+
 | type_CongEq Γ s A1 A2 u1 u2 v1 v2 pA pu pv :
     Σ ;;; Γ |-i pA : sHeq (sSort s) A1 (sSort s) A2 ->
     Σ ;;; Γ |-i pu : sHeq A1 u1 A2 u2 ->
